src/Machine.v
@@ -11,17 +11,21 @@ Set Implicit Arguments.
 
 Module ExecUnit.
   Inductive t := mk {
-    lang: State.t;
+    state: State.t;
     local: Local.t;
     mem: Memory.t;
   }.
   Hint Constructors t.
 
   Inductive step (tid:Id.t) (eu1 eu2:t): Prop :=
-  | step_intro
+  | step_exec
       e
-      (STATE: State.step e eu1.(lang) eu2.(lang))
+      (STATE: State.step e eu1.(state) eu2.(state))
       (LOCAL: Local.step e tid eu1.(local) eu1.(mem) eu2.(local) eu2.(mem))
+  | step_promise
+      loc val
+      (STATE: eu1.(state) = eu2.(state))
+      (LOCAL: Local.promise loc val tid eu1.(local) eu1.(mem) eu2.(local) eu2.(mem))
   .
 End ExecUnit.
 
@@ -39,13 +43,17 @@ Module Machine.
       (STEP: ExecUnit.step tid (ExecUnit.mk st1 lc1 th1.(mem)) (ExecUnit.mk st2 lc2 th2.(mem)))
       (ADD: th2.(tpool) = IdMap.add tid (st2, lc2) th1.(tpool))
   .
+  Hint Constructors step.
 
   (* The consistency condition for the "lazy" semantics. *)
-  Definition consistent (th:t): Prop :=
-    exists th',
-      <<STEP: rtc step th th'>> /\
-      <<PROMISES:
-        forall tid st lc
-          (FIND: IdMap.find tid th'.(tpool) = Some (st, lc)),
-          IdSet.is_empty lc.(Local.promises)>>.
+  Inductive consistent (th:t): Prop :=
+  | consistent_intro
+      th'
+      (STEP: rtc step th th')
+      (PROMISES:
+         forall tid st lc
+           (FIND: IdMap.find tid th'.(tpool) = Some (st, lc)),
+           Promises.is_empty lc.(Local.promises))
+  .
+  Hint Constructors consistent.
 End Machine.
